Impl.fst
@@ -1,5 +1,7 @@
 module Impl
 
+include Impl.Core
+include Impl.Common
 include Impl.Trees
 include Impl.Trees.Rotate
 include Impl.Trees.Rotate2
